WIP
WIP

WIP

WIP

WIP

WIP

WIP

Debugging

WIP

WIP

WIP

WIP

WIP

WIP

WIP

WIP

WIP

WIP

WIP

WIP

WIP

WIP

WIP

WIP

WIP

WIP

WIP

WIP

WIP

WIP

WIP

WIP

Add bound_op

WIP

WIP

WIP

copy_bounds, fill_template

WIP

WIP

WIP

Fix bugs in shr

WIP

WIP

copy_bounds, fill_templates

Add LadderStepDisplay

copy_bounds

Add more notations

Copy bounds

Fix bounds

More notations

C code

More notations for fewer casts

Update log, fix shr

Don't insert identity casts

Update log with elimination of identity casts

Remove useless + casts

Remove useless & casts

Update 32-bit ladder step

Various small notation fixes

Add print of 32-bit ladder

Fix binary notation in 32-bit

Update notations

Update MulDisplay

Add display target

Update notations import

Update notations import

Update display target

Add a bunch of C display files

Remove lowercase files

Add MapBounds

Add 41417 MulDisplay

WIP

Add ComputeBounds

WIP

More/better C notations

Some binary things, remove extra notation

Add Java notations

Remove Java

Hopefully better java display targets

Add Java display things

Add more java display

Add src/SpecificGen/GF25519_64Reflective/Reified/LadderStepJavaDisplay.log

Add more java logs

Constant notation fixes

Add comment about Java casts

davidben tells me unsigned short is bigger than uint8_t

More notations fixes

Fix constants in display

Add more java display

Update display

WIP

WIP

Add TODO

Update TODO

Add to TODO

WIP on good bounds

WIP on good bounds

WIP on good bounds

WIP

WIP

WIP

WIP

Add Z.log2_up_nonneg to zarith

Add valid_update lemmas about FixedWordSizes

WIP

WIP

src/Reflection/Z/Syntax.v
@@ -1,7 +1,10 @@
 (** * PHOAS Syntax for expression trees on ℤ *)
 Require Import Coq.ZArith.ZArith.
+Require Import Bedrock.Word.
 Require Import Crypto.Reflection.Syntax.
 Require Import Crypto.ModularArithmetic.ModularBaseSystemListZOperations.
+Require Import Crypto.Util.FixedWordSizes.
+Require Import Crypto.Util.NatUtil. (* for nat_beq for equality schemes *)
 Export Syntax.Notations.
 
 Local Set Boolean Equality Schemes.
@@ -10,7 +13,8 @@ Inductive base_type := TZ | TWord (logsz : nat).
 
 Definition interp_base_type (v : base_type) : Type :=
   match v with
-  | _ => Z
+  | TZ => Z
+  | TWord logsz => wordT logsz
   end.
 
 Inductive op : flat_type base_type -> flat_type base_type -> Type :=
@@ -29,11 +33,13 @@ Inductive op : flat_type base_type -> flat_type base_type -> Type :=
 
 Definition interpToZ {t} : interp_base_type t -> Z
   := match t with
-     | _ => fun x => x
+     | TZ => fun x => x
+     | TWord _ => wordToZ
      end.
 Definition ZToInterp {t} : Z -> interp_base_type t
   := match t return Z -> interp_base_type t with
-     | _ => fun x => x
+     | TZ => fun x => x
+     | TWord _ => ZToWord
      end.
 Definition cast_const {t1 t2} (v : interp_base_type t1) : interp_base_type t2
   := ZToInterp (interpToZ v).
@@ -45,15 +51,25 @@ Local Notation eta4 x := (eta3 (fst x), snd x).
 Definition interp_op src dst (f : op src dst) : interp_flat_type interp_base_type src -> interp_flat_type interp_base_type dst
   := match f in op src dst return interp_flat_type interp_base_type src -> interp_flat_type interp_base_type dst with
      | OpConst _ v => fun _ => v
-     | Add _ => fun xy => fst xy + snd xy
-     | Sub _ => fun xy => fst xy - snd xy
-     | Mul _ => fun xy => fst xy * snd xy
-     | Shl _ => fun xy => Z.shiftl (fst xy) (snd xy)
-     | Shr _ => fun xy => Z.shiftr (fst xy) (snd xy)
-     | Land _ => fun xy => Z.land (fst xy) (snd xy)
-     | Lor _ => fun xy => Z.lor (fst xy) (snd xy)
-     | Neg _ int_width => fun x => ModularBaseSystemListZOperations.neg int_width x
-     | Cmovne _ => fun xyzw => let '(x, y, z, w) := eta4 xyzw in cmovne x y z w
-     | Cmovle _ => fun xyzw => let '(x, y, z, w) := eta4 xyzw in cmovl x y z w
+     | Add TZ => fun xy => fst xy + snd xy
+     | Sub TZ => fun xy => fst xy - snd xy
+     | Mul TZ => fun xy => fst xy * snd xy
+     | Shl TZ => fun xy => Z.shiftl (fst xy) (snd xy)
+     | Shr TZ => fun xy => Z.shiftr (fst xy) (snd xy)
+     | Land TZ => fun xy => Z.land (fst xy) (snd xy)
+     | Lor TZ => fun xy => Z.lor (fst xy) (snd xy)
+     | Neg TZ int_width => fun x => ModularBaseSystemListZOperations.neg int_width x
+     | Cmovne TZ => fun xyzw => let '(x, y, z, w) := eta4 xyzw in cmovne x y z w
+     | Cmovle TZ => fun xyzw => let '(x, y, z, w) := eta4 xyzw in cmovl x y z w
+     | Add _ => fun xy => wadd (fst xy) (snd xy)
+     | Sub _ => fun xy => wsub (fst xy) (snd xy)
+     | Mul _ => fun xy => wmul (fst xy) (snd xy)
+     | Shl _ => fun xy => wshl (fst xy) (snd xy)
+     | Shr _ => fun xy => wshr (fst xy) (snd xy)
+     | Land _ => fun xy => wland (fst xy) (snd xy)
+     | Lor _ => fun xy => wlor (fst xy) (snd xy)
+     | Neg _ int_width => fun x => ModularBaseSystemListZOperations.wneg int_width x
+     | Cmovne _ => fun xyzw => let '(x, y, z, w) := eta4 xyzw in wcmovne x y z w
+     | Cmovle _ => fun xyzw => let '(x, y, z, w) := eta4 xyzw in wcmovl x y z w
      | Cast _ _ => cast_const
      end%Z.
