src/Reflection/Z/Interpretations.v
@@ -1,0 +1,1473 @@
+(** * Interpretation of PHOAS syntax for expression trees on ℤ *)
+Require Import Coq.ZArith.ZArith.
+Require Import Coq.micromega.Psatz.
+Require Import Crypto.Reflection.Z.Syntax.
+Require Import Crypto.Reflection.Z.Syntax.Util.
+Require Import Crypto.Reflection.Z.OpInversion.
+Require Import Crypto.Reflection.Syntax.
+Require Import Crypto.Reflection.Z.BoundsInterpretations.
+Require Import Crypto.Reflection.Relations.
+Require Import Crypto.Reflection.Wf.
+Require Import Crypto.Reflection.InterpWfRel.
+Require Import Crypto.Reflection.WfProofs.
+Require Import Crypto.Reflection.WfInversion.
+Require Import Crypto.Reflection.SmartMap.
+Require Import Crypto.Reflection.ExprInversion.
+Require Import Crypto.Reflection.TypeInversion.
+Require Import Crypto.Reflection.Linearize.
+Require Import Crypto.Reflection.LinearizeInterp.
+Require Import Crypto.Reflection.LinearizeWf.
+Require Import Crypto.Reflection.Inline.
+Require Import Crypto.Reflection.InlineInterp.
+Require Import Crypto.Reflection.Equality.
+Require Import Crypto.Reflection.MapCast.
+Require Import Crypto.Reflection.MapCastInterp.
+Require Import Crypto.Reflection.MapCastWf.
+Require Import Crypto.Reflection.Eta.
+Require Import Crypto.Reflection.EtaInterp.
+Require Import Crypto.Reflection.SmartBound.
+Require Import Crypto.Reflection.SmartCast.
+Require Import Crypto.Reflection.SmartCastWf.
+Require Import Crypto.Reflection.BoundByCast.
+Require Import Crypto.Reflection.BoundByCastWf.
+Require Import Crypto.Reflection.BoundByCastInterp.
+Require Import Crypto.ModularArithmetic.ModularBaseSystemListZOperations.
+Require Import Crypto.Util.Equality.
+Require Import Crypto.Util.Sigma.
+Require Import Crypto.Util.Prod.
+Require Import Crypto.Util.NatUtil.
+Require Import Crypto.Util.ZUtil.
+Require Import Crypto.Util.Option.
+Require Crypto.Util.Tuple.
+Require Crypto.Util.HList.
+Require Import Crypto.Util.Bool.
+Require Import Crypto.Util.Prod.
+Require Import Crypto.Util.Tactics.
+Require Import Bedrock.Word.
+Require Import Crypto.Util.WordUtil.
+Require Import Crypto.Util.FixedWordSizesEquality.
+Export Reflection.Syntax.Notations.
+
+Local Notation eta x := (fst x, snd x).
+Local Notation eta3 x := (eta (fst x), snd x).
+Local Notation eta4 x := (eta3 (fst x), snd x).
+
+Module Import Bounds.
+  Import BoundsInterpretations.Bounds.
+  Import Bounds.Notations.
+
+  Definition ComputeBounds {t} (e : Expr base_type op t)
+             (input_bounds : interp_flat_type Bounds.interp_base_type (domain t))
+    : interp_flat_type Bounds.interp_base_type (codomain t)
+    := Interp (@Bounds.interp_op) e input_bounds.
+
+  Definition map_uncast_const {t} (bounds : interp_flat_type Bounds.interp_base_type t) (e : interp_flat_type Syntax.interp_base_type _)
+    : interp_flat_type Syntax.interp_base_type t
+    := interpf_smart_unbound
+         Bounds.interp_base_type (fun _ => @Bounds.bounds_to_base_type)
+         (@cast_const)
+         bounds e.
+
+  Local Notation bound_base_type t := Bounds.bounds_to_base_type (only parsing).
+
+  Local Hint Extern 1 => progress simpl.
+  Local Hint Extern 1 (_ = _) => reflexivity.
+  Local Hint Resolve cast_const_id @cast_const_idempotent.
+  Local Arguments Z.pow_pos !_ !_ / .
+  Local Arguments Z.add !_ !_.
+  Section with_rewrite_le.
+    Local Existing Instances Z.add_le_Proper Z.sub_le_eq_Proper Z.log2_up_le_Proper Z.pow_Zpos_le_Proper.
+    Lemma strip_cast_const t x y
+      : @Bounds.is_bounded_by' t y x
+        -> @cast_const (bound_base_type t x) t (@cast_const t (bound_base_type t x) y) = y.
+    Proof.
+      unfold Bounds.is_bounded_by', Bounds.is_bounded_byb, cast_const, ZToInterp, interpToZ.
+      repeat first [ progress subst
+                   | reflexivity
+                   | congruence
+                   | progress destruct_head_hnf' option
+                   | progress destruct_head_hnf' bounds
+                   | progress destruct_head_hnf' base_type
+                   | progress Z.ltb_to_lt
+                   | progress split_andb
+                   | progress unfold bounds_to_base_type' in *
+                   | progress intros
+                   | match goal with
+                     | [ H : TWord _ = TWord _ |- _ ] => inversion H; clear H
+                     | [ |- (?x < ?y)%Z ]
+                       => cut (x <= y - 1)%Z; [ omega | ]
+                     end
+                   | progress rewrite ?wordToZ_ZToWord, ?ZToWord_wordToZ, ?ZToWord_gen_wordToZ_gen, ?Z.pow_Zpow
+                   | rewrite Z2Nat.id by auto with zarith
+                   | progress break_innermost_match_step
+                   | progress break_match_hyps
+                   | rewrite <- !Z.log2_up_le_full
+                   | progress simpl in *
+                   | omega
+                   | split; [ reflexivity || omega | ] ].
+    Qed.
+  End with_rewrite_le.
+
+  Local Notation bound_op := (@bound_op _ _ _ (@Bounds.interp_op) (fun t => bound_base_type t) _ internal_base_type_dec_bl base_type_leb (@Castb) genericize_op).
+  Local Notation G_invariant_holds G
+    := (forall t x x',
+           List.In (existT _ t (x, x')%core) G -> @is_bounded_by' t x x')
+         (only parsing).
+
+  Section bounded_by_interp_op.
+    Local Notation is_bounded_by_interp_opT opc
+      := (forall t sv1 sv2,
+             is_bounded_by sv1 sv2
+             -> is_bounded_by (Syntax.interp_op _ _ (opc t) sv1) (interp_op (opc t) sv2))
+           (only parsing).
+    Local Notation is_bounded_by_bound_opT opc
+      := (forall
+             t G ein eout ebounds
+             (Hwf : wff G ein ebounds)
+             (HG : G_invariant_holds G)
+             (Hinout : interpf Syntax.interp_op ein = interpf Syntax.interp_op eout)
+             (Hrgood : bounds_are_recursively_good (@Bounds.interp_op) bound_is_good ebounds)
+             (Hgood : bounds_are_good (@Bounds.interp_op _ _ (opc t) (interpf (@Bounds.interp_op) ebounds))),
+             is_bounded_by
+               (interpf Syntax.interp_op (@bound_op Syntax.interp_base_type _ _ _ _ (opc t) (opc t) eout (interpf (@Bounds.interp_op) ebounds)))
+               (interpf (@Bounds.interp_op) (Op (opc t) ebounds)))
+           (only parsing).
+
+    Local Notation interpf_bound_opT opc
+      := (forall t G ein eout ebounds
+                 (Hwf : wff G ein ebounds)
+                 (HG : G_invariant_holds G)
+                 (Hinout : interpf Syntax.interp_op ein = interpf Syntax.interp_op eout)
+                 (Hrgood : bounds_are_recursively_good (@Bounds.interp_op) bound_is_good ebounds)
+                 (Hgood : bounds_are_good (@Bounds.interp_op _ _ (opc t) (interpf (@Bounds.interp_op) ebounds))),
+             interpf Syntax.interp_op (@bound_op Syntax.interp_base_type _ _ _ _ (opc t) (opc t) eout (interpf (@Bounds.interp_op) ebounds))
+             = interpf Syntax.interp_op (Op (opc t) ein))
+           (only parsing).
+
+    Local Ltac fin_t :=
+      first [ reflexivity
+            | omega
+            | match goal with |- context[(_ * _)%Z] => idtac end;
+              nia ].
+
+    Local Ltac intro_t :=
+      first [ progress simpl in *
+            | progress intros ].
+
+    Local Ltac break1_t :=
+      first [ progress subst
+            | progress destruct_head_hnf' unit
+            | progress inversion_bounds
+            | progress inversion_option
+            | progress destruct_head' and
+            | progress destruct_head' prod
+            | progress destruct_head_hnf' bounds
+            | progress split_andb
+            | progress split_and ].
+    Local Ltac break2_t :=
+      first [ progress destruct_head' base_type
+            | progress destruct_head_hnf' option
+            | progress destruct_head' or
+            | progress break_innermost_match_step ].
+    Local Ltac unfolder_t :=
+      first [ progress unfold is_bounded_by', is_bounded_byb in *
+            | progress unfold SmartBuildBounds, SmartVarfMap in *
+            | progress unfold neg, cmovle, cmovne in *
+            | progress unfold ModularBaseSystemListZOperations.wneg, ModularBaseSystemListZOperations.neg, ModularBaseSystemListZOperations.wcmovne, ModularBaseSystemListZOperations.cmovne, ModularBaseSystemListZOperations.wcmovl, ModularBaseSystemListZOperations.cmovl in * ].
+    Local Ltac late_unfolder_t :=
+      first [ progress unfold wneg_gen, wcmovl_gen, wcmovne_gen in * ].
+
+    (* split the goal, but only if it's about Z, not word *)
+    Local Ltac Z_andb_splitter_t :=
+      lazymatch goal with
+      | [ sz : nat |- _ ] => fail
+      | [ w : FixedWordSizes.wordT _ |- _ ] => fail
+      | [ w : word _ |- _ ] => fail
+      | [ |- andb _ _ = true ] => apply Bool.andb_true_iff, conj
+      end.
+
+    Local Ltac rewriter1_t :=
+      match goal with
+      | [ H : true = true |- _ ] => clear H
+      | [ H : ?x = true, H' : context[?x] |- _ ] => rewrite H in H'
+      | [ H : ?x = true |- context[?x] ] => rewrite H
+      | _ => rewrite Bool.andb_true_r
+      | _ => rewrite Bool.andb_true_l
+      | [ H : andb _ _ = false |- _ ] => apply Bool.andb_false_iff in H
+      | _ => rewrite wordToZ_gen_ZToWord_gen
+          by (rewrite ?Z.pow_Zpow; eauto using Z.ones_nonneg, (fun a b pf => proj2 (Z.log2_lt_pow2_alt a b pf)), Z.le_lt_trans, Z.log2_nonneg with omega)
+      | _ => rewrite wordToZ_ZToWord
+          by (rewrite ?Z.pow_Zpow; eauto using Z.ones_nonneg, (fun a b pf => proj2 (Z.log2_lt_pow2_alt a b pf)), Z.le_lt_trans, Z.log2_nonneg with omega)
+      end.
+
+    Local Ltac Zltb_to_lt :=
+      first [ progress Z.ltb_to_lt
+            | match goal with
+              | [ |- ((_ <=? _) && (_ <=? _))%Z%bool = true ]
+                => rewrite Bool.andb_true_iff, !Z.leb_le
+              end ].
+
+    Local Ltac simpler_t :=
+      first [ progress specialize_by auto
+            | match goal with
+              | [ H : context[Z.of_N (wordToN ?x)] |- _ ]
+                => change (Z.of_N (wordToN x)) with (FixedWordSizes.wordToZ_gen x) in *
+              | [ |- context[Z.of_N (wordToN ?x)] ]
+                => change (Z.of_N (wordToN x)) with (FixedWordSizes.wordToZ_gen x) in *
+              | [ H : (?x <= ?x)%Z |- _ ] => clear H
+              | [ H : FixedWordSizes.wordToZ ?x = _ |- _ ]
+                => generalize dependent (FixedWordSizes.wordToZ x); clear x; intros; subst
+              | [ H : _ = FixedWordSizes.wordToZ ?x |- _ ]
+                => generalize dependent (FixedWordSizes.wordToZ x); clear x; intros; subst
+              end ].
+
+    Local Ltac misc_solver_t :=
+      solve [ eauto using Z.shiftl_le_mono, Z.shiftr_le_mono, Z.ones_nonneg with nocore omega
+            | apply Z.land_nonneg; eauto with nocore omega
+            | apply Z.min_case_strong;
+              eauto using Z.land_upper_bound_r, Z.land_upper_bound_l, Z.le_trans with nocore omega
+            | apply Z.lor_bounds_gen_lower; eauto using Z.max_le_compat with omega
+            | autorewrite with push_Zmax;
+              apply Z.lor_bounds_gen_upper; eauto using Z.le_max_l, Z.le_max_r, Z.le_trans with omega
+            | apply Z.max_case_strong; omega ].
+
+    Local Ltac t_step :=
+      first [ fin_t
+            | intro_t
+            | break1_t
+            | unfolder_t
+            | rewriter1_t
+            | simpler_t
+            | Z_andb_splitter_t
+            | break2_t
+            | Zltb_to_lt
+            | progress adjust_mbs_wops
+            | misc_solver_t
+            | progress syntactic_fixed_size_op_to_word
+            | late_unfolder_t ].
+    Local Ltac t := repeat t_step.
+
+    Local Ltac precutZ :=
+      let G := match goal with |- forall t, @?G t => G end in
+      let t := fresh in
+      intro t;
+      cut (G TZ);
+      [ destruct t; [ solve [ trivial ]
+                    | ]
+      | clear t ].
+    Local Ltac cutZ :=
+      precutZ;
+      [ let H := fresh in
+        let b := fresh in
+        let v := fresh in
+        intros H v b;
+        specialize (H (SmartVarfMap (fun _ => interpToZ) v) b)
+      | ].
+
+    Lemma add_is_bounded_by_interp_op : is_bounded_by_interp_opT Add.
+    Proof. cutZ; t. split; eapply wadd_valid_update; eauto. Qed.
+    Local Hint Resolve add_is_bounded_by_interp_op.
+    Lemma sub_is_bounded_by_interp_op : is_bounded_by_interp_opT Sub.
+    Proof. cutZ; t. split; eapply wsub_valid_update; eauto. Qed.
+    Local Hint Resolve sub_is_bounded_by_interp_op.
+    Lemma mul_is_bounded_by_interp_op : is_bounded_by_interp_opT Mul.
+    Proof. cutZ; t. split; eapply wmul_valid_update; eauto. Qed.
+    Local Hint Resolve mul_is_bounded_by_interp_op.
+    Lemma shl_is_bounded_by_interp_op : is_bounded_by_interp_opT Shl.
+    Proof. cutZ; t. split; eapply wshl_valid_update; eauto. Qed.
+    Local Hint Resolve shl_is_bounded_by_interp_op.
+    Lemma shr_is_bounded_by_interp_op : is_bounded_by_interp_opT Shr.
+    Proof. cutZ; t. split; eapply wshr_valid_update; eauto. Qed.
+    Local Hint Resolve shr_is_bounded_by_interp_op.
+    Lemma land_is_bounded_by_interp_op : is_bounded_by_interp_opT Land.
+    Proof. cutZ; t. split; eapply wland_valid_update; eauto with omega. Qed.
+    Local Hint Resolve land_is_bounded_by_interp_op.
+    Lemma lor_is_bounded_by_interp_op : is_bounded_by_interp_opT Lor.
+    Proof. cutZ; t. split; eapply wlor_valid_update; eauto. Qed.
+    Local Hint Resolve lor_is_bounded_by_interp_op.
+    Lemma neg_is_bounded_by_interp_op int_size : is_bounded_by_interp_opT (fun T => Neg T int_size).
+    Proof. cutZ; t. Qed.
+    Local Hint Resolve neg_is_bounded_by_interp_op.
+    Lemma cmovne_is_bounded_by_interp_op : is_bounded_by_interp_opT Cmovne.
+    Proof. cutZ; t. Qed.
+    Local Hint Resolve cmovne_is_bounded_by_interp_op.
+    Lemma cmovle_is_bounded_by_interp_op : is_bounded_by_interp_opT Cmovle.
+    Proof. cutZ; t. Qed.
+    Local Hint Resolve cmovle_is_bounded_by_interp_op.
+    Lemma cast_is_bounded_by_interp_op T : is_bounded_by_interp_opT (Cast T).
+    Proof. t. Qed.
+    Local Hint Resolve cast_is_bounded_by_interp_op.
+
+    Lemma is_bounded_by_interp_op src dst (op : op src dst)
+      : forall (sv1 : interp_flat_type Syntax.interp_base_type src)
+               (sv2 : interp_flat_type interp_base_type src)
+               (H : is_bounded_by sv1 sv2),
+        is_bounded_by (Syntax.interp_op src dst op sv1) (interp_op op sv2).
+    Proof.
+      destruct op; auto.
+      { (* const casse *) t. }
+    Qed.
+
+    Local Hint Resolve @is_bounded_by_interp_op.
+
+    Local Ltac misc_t_2 :=
+      match goal with
+      | [ H : _ = _ :> prod _ _ |- _ ]
+        => pose proof (f_equal (@fst _ _) H);
+           pose proof (f_equal (@snd _ _) H);
+           clear H
+      end.
+
+    Local Ltac inequality_t :=
+      match goal with
+      | _ => rewrite Z.pow_Zpow
+      | _ => rewrite Z2Nat.id by auto using Z.log2_up_nonneg
+      | [ |- (_ <= _ < _)%Z ]
+        => split; [ solve [ fin_t ] | ]
+      | [ |- (?x < ?y)%Z ]
+        => cut (x <= y - 1)%Z; [ omega | ]
+      | _ => rewrite <- !Z.log2_up_le_full
+      end.
+
+    Section with_le_instances.
+      Local Arguments Z.add !_ !_.
+      Local Existing Instances Z.add_le_Proper Z.sub_le_eq_Proper Z.log2_up_le_Proper Z.pow_Zpos_le_Proper.
+
+      Lemma add_is_bounded_by_bound_op : is_bounded_by_bound_opT Add.
+      Proof. precutZ.
+             intros H G ein eout ebounds Hwf HG Hinout Hrgood Hgood;
+               specialize (H G);
+               revert dependent ein; intro ein; revert dependent eout; intro eout;
+                 revert dependent ebounds; revert ein eout;
+                   do 3 (intro;
+                         let e := lazymatch goal with e : _ |- _ => e end in
+                         let TZ := match type of H with forall a : exprf _ _ ?T, _ => T end in
+                         let TW := match type of e with exprf _ _ ?T => T end in
+                         specialize (H (LetIn e
+                                              (invert_Some (@SmartCast.SmartCast _ op _ internal_base_type_dec_bl (@Castb) _ TW TZ)))));
+                   intros.
+             let T := match type of H with ?T -> _ => T end in
+             let H' := fresh in
+             assert (H' : T); [ | specialize (H H'); clear H' ].
+             { constructor; auto; intros.
+               eapply wff_in_impl_Proper.
+               { lazymatch goal with
+                 | [ |- wff (var1:=?var1) (var2:=?var2) ?G
+                            (invert_Some (SmartCast _ _ _ ?TW ?TZ) ?x)
+                            (invert_Some (SmartCast _ _ _ ?TW ?TZ) ?y) ]
+                   => exact (@wff_SmartCast_match _ op _ internal_base_type_dec_bl (@Castb) (@wff_Castb) var1 var2 TW TZ x y)
+                 end. }
+               { intros; rewrite List.in_app_iff; auto. } }
+             specialize_by auto.
+             simpl in H.
+             rewrite Hinout in H.
+             specialize_by reflexivity.
+
+             repeat (specialize (fun a b => H (conj a b)); specialize_by auto).
+               (*
+             specialize_by eauto with wf.
+                   pose (LetIn ein Cst) as ein';
+                   pose (LetIn ein Cst) as eout';
+                   pose (LetIn ein Cst) as ebounds'.
+             Focus 2.
+             simpl.
+             { cbv [LetIn.Let_In].
+               intros.
+               pose proof Hwf as Hwf'.
+               eapply interpf_wff with (R:=@is_bounded_by') in Hwf';
+                 [ | solve [ apply is_bounded_by_interp_op ] | solve [ auto ] ].
+               unfold bound_is_good in Hgood.
+               unfold bound_is_goodb in Hgood.
+               break_match_hyps; try congruence.
+               simpl in * |- .
+               unfold is_bounded_by' in *.
+               unfold bounds_to_base_type.
+               unfold bounds_to_base_type'.
+               unfold SmartCast.SmartCast_base.
+               destruct_head' and.
+               repeat break_innermost_match; simpl in *; try congruence.
+               Focus 2.
+               { unfold add in *.
+                 unfold is_bounded_byb in *.
+                 unfold t_map2 in *.
+                 unfold add' in *.
+                 unfold SmartBuildBounds in *.
+                 break_match_hyps; inversion_option; subst; simpl in *; split_andb; congruence. }
+               Unfocus.
+               rewrite_hyp !*; simpl.
+               unfold add in *.
+               Locate wadd_def_ZToWord.
+               rewrite wadd_def_ZToWord.
+               Focus 2.
+               { unfold t_map2, add', SmartBuildBounds, is_bounded_byb in *.
+                 break_match_hyps; simpl in *; inversion_option; split_andb; subst; simpl in *.
+                 Z.ltb_to_lt.
+                 rewrite !wordToZ_ZToWord by repeat (t || misc_t_2 || inequality_t).
+                 repeat (t || misc_t_2 || inequality_t). }
+               Unfocus.
+               { repeat (t || misc_t_2 || inequality_t || break_match_hyps).
+                 all:destruct (interpf Syntax.interp_op ein) as [x y]; simpl in *; subst.
+                 all:destruct (interpf Syntax.interp_op eout) as [x y]; simpl in *; subst.
+                 { repeat rewrite !wordToZ_ZToWord; repeat (t || misc_t_2 || inequality_t || break_match_hyps). }
+                 { repeat rewrite !wordToZ_ZToWord; repeat (t || misc_t_2 || inequality_t || break_match_hyps). } } }
+             Unfocus.
+             Print SmartBound.
+             .
+             simpl in *.
+             cbv [LetIn.Let_In] in *.
+             unfold SmartCast.SmartCast_base in *.
+               t.
+                 destruct (interpf Syntax.interp_op eout) as [x y]; simpl in *; subst.
+                 destruct (interpf Syntax.interp_op ein) as [x y]; simpl in *.
+                 destruct (Z_zerop upper1), (Z_zerop upper0); subst; simpl;
+                   try assert (x = 0%Z) by omega;
+                   try assert (y = 0%Z) by omega;
+                   subst; simpl;
+                     try rewrite Z.log2_up_eqn by omega;
+                     rewrite <- ?Z.add_1_r, <- ?Z.sub_1_r;
+                     autorewrite with zsimplify;
+                     try (apply Z.log2_le_mono; omega).
+                 SearchAbout Z.pred (-1 )%Z.
+                 Focus 2.
+                 SearchAbout Z.log2 Z.log2_up.
+                 Focus 2.
+                 { repeat (t || misc_t_2 || inequality_t). }
+                 Unfocus.
+                 Typeclasses eauto := debug.
+                 Import Morphisms RelationClasses.
+                 pose proof (_ : Proper (_ ==> Z.le --> _) Z.pow).
+                 try rewrite <- Z.log2_up_le_full.
+                 pose
+
+
+                 Set Printing Coercions.
+                 .
+                 Focus 2.
+                 { t.
+                   .
+               .
+             SearchAbout FixedWordSizes.wadd.
+             rewrite Heqb0.
+             unfold is_bounded_byb.*)
+    Admitted.
+    Local Hint Resolve add_is_bounded_by_bound_op.
+    Lemma sub_is_bounded_by_bound_op : is_bounded_by_bound_opT Sub.
+    Proof. precutZ. Admitted.
+    Local Hint Resolve sub_is_bounded_by_bound_op.
+    Lemma mul_is_bounded_by_bound_op : is_bounded_by_bound_opT Mul.
+    Proof. precutZ. Admitted.
+    Local Hint Resolve mul_is_bounded_by_bound_op.
+    Lemma shl_is_bounded_by_bound_op : is_bounded_by_bound_opT Shl.
+    Proof. precutZ. Admitted.
+    Local Hint Resolve shl_is_bounded_by_bound_op.
+    Lemma shr_is_bounded_by_bound_op : is_bounded_by_bound_opT Shr.
+    Proof. precutZ. Admitted.
+    Local Hint Resolve shr_is_bounded_by_bound_op.
+    Lemma land_is_bounded_by_bound_op : is_bounded_by_bound_opT Land.
+    Proof. precutZ. Admitted.
+    Local Hint Resolve land_is_bounded_by_bound_op.
+    Lemma lor_is_bounded_by_bound_op : is_bounded_by_bound_opT Lor.
+    Proof. precutZ. Admitted.
+    Local Hint Resolve lor_is_bounded_by_bound_op.
+    Lemma neg_is_bounded_by_bound_op int_size : is_bounded_by_bound_opT (fun T => Neg T int_size).
+    Proof. precutZ.
+           intros H G ein eout ebounds Hwf HG Hinout Hrgood Hgood;
+             specialize (H G).
+           Focus 2.
+           { simpl. t.
+    Admitted.
+    Local Hint Resolve neg_is_bounded_by_bound_op.
+    Lemma cmovne_is_bounded_by_bound_op : is_bounded_by_bound_opT Cmovne.
+    Proof. precutZ. Admitted.
+    Local Hint Resolve cmovne_is_bounded_by_bound_op.
+    Lemma cmovle_is_bounded_by_bound_op : is_bounded_by_bound_opT Cmovle.
+    Proof. precutZ. Admitted.
+    Local Hint Resolve cmovle_is_bounded_by_bound_op.
+    Lemma cast_is_bounded_by_bound_op T : is_bounded_by_bound_opT (Cast T).
+    Proof. precutZ. Admitted.
+    Local Hint Resolve cast_is_bounded_by_bound_op.
+
+    Lemma is_bounded_by_bound_op
+          G t tR (opc : op t tR) ein eout ebounds
+          (Hwf : wff G ein ebounds)
+          (HG : G_invariant_holds G)
+          (Hinout : interpf Syntax.interp_op ein = interpf Syntax.interp_op eout)
+          (Hrgood : bounds_are_recursively_good (@Bounds.interp_op) bound_is_good ebounds)
+          (Hgood : bounds_are_good (@Bounds.interp_op _ _ opc (interpf (@Bounds.interp_op) ebounds)))
+      : is_bounded_by
+          (interpf Syntax.interp_op (@bound_op Syntax.interp_base_type _ _ _ _ opc opc eout (interpf (@Bounds.interp_op) ebounds)))
+          (interpf (@Bounds.interp_op) (Op opc ebounds)).
+    Proof.
+      destruct opc; eauto.
+      { (* const casse *) t. }
+    Qed.
+
+
+    Lemma add_interpf_bound_op : interpf_bound_opT Add.
+    Proof. precutZ.
+           intros H G ein eout ebounds Hwf HG Hinout Hrgood Hgood;
+             specialize (H G). Admitted.
+    Local Hint Resolve add_interpf_bound_op.
+    Lemma sub_interpf_bound_op : interpf_bound_opT Sub.
+    Proof. precutZ. Admitted.
+    Local Hint Resolve sub_interpf_bound_op.
+    Lemma mul_interpf_bound_op : interpf_bound_opT Mul.
+    Proof. precutZ. Admitted.
+    Local Hint Resolve mul_interpf_bound_op.
+    Lemma shl_interpf_bound_op : interpf_bound_opT Shl.
+    Proof. precutZ. Admitted.
+    Local Hint Resolve shl_interpf_bound_op.
+    Lemma shr_interpf_bound_op : interpf_bound_opT Shr.
+    Proof. precutZ. Admitted.
+    Local Hint Resolve shr_interpf_bound_op.
+    Lemma land_interpf_bound_op : interpf_bound_opT Land.
+    Proof. precutZ. Admitted.
+    Local Hint Resolve land_interpf_bound_op.
+    Lemma lor_interpf_bound_op : interpf_bound_opT Lor.
+    Proof. precutZ. Admitted.
+    Local Hint Resolve lor_interpf_bound_op.
+    Lemma neg_interpf_bound_op int_size : interpf_bound_opT (fun T => Neg T int_size).
+    Proof. precutZ.
+           intros H G ein eout ebounds Hwf HG Hinout Hrgood Hgood;
+             specialize (H G).
+           Focus 2.
+           { simpl. t.
+    Admitted.
+    Local Hint Resolve neg_interpf_bound_op.
+    Lemma cmovne_interpf_bound_op : interpf_bound_opT Cmovne.
+    Proof. precutZ. Admitted.
+    Local Hint Resolve cmovne_interpf_bound_op.
+    Lemma cmovle_interpf_bound_op : interpf_bound_opT Cmovle.
+    Proof. precutZ. Admitted.
+    Local Hint Resolve cmovle_interpf_bound_op.
+    Lemma cast_interpf_bound_op T : interpf_bound_opT (Cast T).
+    Proof. simpl; congruence. Qed.
+    Local Hint Resolve cast_interpf_bound_op.
+
+    Lemma interpf_bound_op
+          G t tR (opc : op t tR) ein eout ebounds
+          (Hwf : wff G ein ebounds)
+          (HG : G_invariant_holds G)
+          (Hinout : interpf Syntax.interp_op ein = interpf Syntax.interp_op eout)
+          (Hrgood : bounds_are_recursively_good (@Bounds.interp_op) bound_is_good ebounds)
+          (Hgood : bounds_are_good (@Bounds.interp_op _ _ opc (interpf (@Bounds.interp_op) ebounds)))
+      : interpf Syntax.interp_op (@bound_op Syntax.interp_base_type t tR t tR opc opc eout (interpf (@Bounds.interp_op) ebounds))
+        = interpf Syntax.interp_op (Op opc ein).
+    Proof.
+      destruct opc; eauto.
+    Qed.
+    End with_le_instances.
+  End bounded_by_interp_op.
+
+  Local Hint Resolve @is_bounded_by_interp_op @is_bounded_by_bound_op @interpf_bound_op.
+
+  Definition MapBounds {t}
+             (e : Expr base_type op t)
+             (input_bounds : interp_flat_type Bounds.interp_base_type (domain t))
+    : Expr base_type op _
+    := @Boundify
+         base_type op
+         (@Bounds.interp_base_type) (@Bounds.interp_op)
+         (fun _ => bounds_to_base_type)
+         base_type_beq internal_base_type_dec_bl
+         base_type_leb
+         (@Castb)
+         is_cast is_const
+         genericize_op
+         (fun _ t => Op (OpConst (ZToInterp 0)) TT)
+         t e input_bounds.
+
+  Lemma MapBounds_correct_and_bounded {t}
+        (e : Expr base_type op t)
+        (Hwf : Wf e)
+        (input_bounds : interp_flat_type interp_base_type (domain t))
+        (output_bounds := ComputeBounds e input_bounds)
+        (e' := MapBounds e input_bounds)
+        (Hgood : bounds_are_recursively_good
+                   (@interp_op) bound_is_good
+                   (invert_Abs (e interp_base_type) input_bounds))
+    : forall x y,
+      map_uncast_const input_bounds x = y
+      -> is_bounded_by y input_bounds
+      -> is_bounded_by (Interp (@Syntax.interp_op) e y) output_bounds
+         /\ map_uncast_const _ (Interp (@Syntax.interp_op) e' x)
+            = Interp (@Syntax.interp_op) e y.
+  Proof.
+    intros x y ? Hb; subst y output_bounds e'.
+    unfold MapBounds, ComputeBounds.
+    eapply InterpBoundifyAndRel; eauto with wf.
+    { apply is_cast_correct. }
+    { apply strip_cast_const. }
+    { apply is_bounded_by_interp_op. }
+    { apply is_bounded_by_bound_op. }
+  Qed.
+
+  Lemma MapBounds_correct_and_bounded_bool {t}
+        (e : Expr base_type op t)
+        (Hwf : Wf e)
+        (input_bounds : interp_flat_type interp_base_type (domain t))
+        (output_bounds := ComputeBounds e input_bounds)
+        (e' := MapBounds e input_bounds)
+        (Hgood : ((bounds_are_recursively_goodb
+                     (@interp_op) bound_is_goodb
+                     (invert_Abs (e interp_base_type) input_bounds)))%bool
+                 = true)
+    : forall x,
+      is_bounded_by (map_uncast_const input_bounds x) input_bounds
+      -> is_bounded_by (Interp (@Syntax.interp_op) e (map_uncast_const _ x)) output_bounds
+         /\ map_uncast_const _ (Interp (@Syntax.interp_op) e' x)
+            = Interp (@Syntax.interp_op) e (map_uncast_const _ x).
+  Proof.
+    intros; eapply MapBounds_correct_and_bounded; eauto.
+    { apply bounds_are_recursively_good_iff_bool; assumption. }
+  Qed.
+
+
+  (*
+
+
+  Local Notation new_flat_type (*: forall t, interp_flat_type interp_base_type2 t -> flat_type base_type_code1*)
+    := (@SmartFlatTypeMap2 _ _ interp_base_type (fun t v => Tbase (bounds_to_base_type v))).
+  Lemma new_flat_type_Pair {A B} (v : interp_flat_type _ A * interp_flat_type _ B)
+    : @new_flat_type (Prod A B) v = Prod (new_flat_type (fst v)) (new_flat_type (snd v)).
+  Proof. reflexivity. Qed.
+  Local Ltac rewrite_new_flat_type_Pair :=
+    match goal with
+    | [ |- context[@new_flat_type (Prod ?A ?B) ?VVV] ]
+      => progress change (@new_flat_type (Prod A B) VVV) with (Prod (@new_flat_type A (fst VVV)) (@new_flat_type B (snd VVV))) in *
+    | [ H : context[@new_flat_type (Prod ?A ?B) ?VVV] |- _ ]
+      => progress change (@new_flat_type (Prod A B) VVV) with (Prod (@new_flat_type A (fst VVV)) (@new_flat_type B (snd VVV))) in *
+    end.
+  Definition new_type {t}
+    : forall (ve : interp_flat_type interp_base_type (domain t))
+             (v : interp_type interp_base_type t),
+      type base_type
+    := fun ve v => Arrow (@new_flat_type (domain t) ve) (@new_flat_type (codomain t) (v ve)).
+  Definition SmartBoundv {var t} (bounds : interp_flat_type Bounds.interp_base_type t) (e : interp_flat_type var t)
+    : interp_flat_type (fun t => @exprf base_type op var (Tbase t)) (new_flat_type bounds)
+    := SmartFlatTypeMap2Interp2 (f:=fun _ _ => Tbase _) (fun t b v => SmartCast_base (Var v)) bounds e.
+  Definition map_cast_const {t} (bounds : interp_flat_type Bounds.interp_base_type t) (e : interp_flat_type Syntax.interp_base_type t)
+    : interp_flat_type Syntax.interp_base_type (new_flat_type bounds)
+    := SmartFlatTypeMap2Interp2 (f:=fun _ _ => Tbase _) (fun t b v => cast_const v) bounds e.
+  Definition map_uncast_const {t} (bounds : interp_flat_type Bounds.interp_base_type t) (e : interp_flat_type Syntax.interp_base_type (new_flat_type bounds))
+    : interp_flat_type Syntax.interp_base_type t
+    := SmartFlatTypeMapUnInterp2 (f:=fun _ _ => Tbase _) (fun t b v => cast_const v) e.
+  Definition SmartUnboundv {var t} {bounds : interp_flat_type Bounds.interp_base_type t}
+             (e : interp_flat_type var (new_flat_type bounds))
+    : interp_flat_type (fun t => @exprf base_type op var (Tbase t)) t
+    := SmartFlatTypeMapUnInterp2 (f:=fun _ _ => Tbase _) (fun t b (v : var _) => SmartCast_base (Var v)) e.
+  Definition SmartBound {t} (e : Expr base_type op t)
+             (input_bounds : interp_flat_type Bounds.interp_base_type (domain t))
+    : Expr base_type op (new_type input_bounds (Interp (@Bounds.interp_op) e))
+    := fun var => Abs (fun x => LetIn
+                                  (LetIn (SmartPairf (SmartUnboundv x))
+                                         (invert_Abs (e var)))
+                                  (fun v => SmartPairf (SmartBoundv _ v))).
+
+  Lemma map_cast_const_Pair {A B} bounds e
+    : @map_cast_const (Prod A B) bounds e
+      = (map_cast_const (fst bounds) (fst e), map_cast_const (snd bounds) (snd e)).
+  Proof. reflexivity. Qed.
+
+  Lemma map_uncast_const_Pair {A B} bounds e
+    : @map_uncast_const (Prod A B) bounds e
+      = (map_uncast_const (fst bounds) (fst e), map_uncast_const (snd bounds) (snd e)).
+  Proof. reflexivity. Qed.
+
+  Lemma SmartUnboundv_Pair {var A B} bounds e
+    : @SmartUnboundv var (Prod A B) bounds e
+      = (SmartUnboundv (fst e), SmartUnboundv (snd e)).
+  Proof. reflexivity. Qed.
+
+  Lemma SmartBoundv_Pair {var A B} (bounds : interp_flat_type _ _ * interp_flat_type _ _)
+        (e : interp_flat_type _ _ * interp_flat_type _ _)
+    : @SmartBoundv var (Prod A B) bounds e
+      = (SmartBoundv (t:=A) (fst bounds) (fst e), SmartBoundv (t:=B) (snd bounds) (snd e)).
+  Proof. reflexivity. Qed.
+
+  Local Hint Resolve List.in_or_app.
+
+  Lemma wff_SmartUnboundv {var1 var2} t input_bounds
+        (x : interp_flat_type var1 (new_flat_type (t:=t) input_bounds))
+        (x' : interp_flat_type var2 (new_flat_type input_bounds))
+    : wff (flatten_binding_list x x')
+          (SmartPairf (SmartUnboundv x))
+          (SmartPairf (SmartUnboundv x')).
+  Proof.
+    induction t; simpl in *;
+      try rewrite_new_flat_type_Pair;
+      rewrite ?SmartUnboundv_Pair, ?SmartPairf_Pair;
+      try constructor;
+      try solve [ eapply wff_in_impl_Proper; eauto ].
+    { unfold SmartPairf, SmartUnboundv, SmartCast_base; simpl;
+        break_match.
+      { let H := match goal with H : _ = _ |- _ => H end in
+        case H; repeat constructor. }
+      { repeat constructor. } }
+  Qed.
+
+  Local Hint Resolve @wff_SmartUnboundv.
+
+  Lemma wff_SmartBoundv {var1 var2} G t f x1 x2
+        (Hwf : wff (op:=op) G (SmartVarf x1) (SmartVarf x2))
+    : wff (var1:=var1) (var2:=var2) G
+          (SmartPairf (SmartBoundv f x1))
+          (SmartPairf (SmartBoundv (t:=t) f x2)).
+  Proof.
+    induction t; simpl in *;
+      destruct_head' prod;
+      rewrite ?SmartVarf_Pair in Hwf;
+      rewrite ?SmartBoundv_Pair; simpl in *;
+        try setoid_rewrite SmartPairf_Pair;
+        inversion_wf;
+        destruct_head' and;
+        try constructor; eauto.
+    { unfold SmartPairf, SmartBoundv, SmartCast_base, SmartFlatTypeMap2, SmartVarf in *; simpl in *.
+      break_match; repeat (trivial || constructor). }
+  Qed.
+
+  Local Hint Resolve wff_SmartBoundv.
+
+  Local Hint Resolve wff_SmartVarf.
+
+  Lemma Wf_SmartBound {t} e input_bounds
+        (Hwf : Wf e)
+    : Wf (@SmartBound t e input_bounds).
+  Proof.
+    intros var1 var2; specialize (Hwf var1 var2).
+    unfold SmartBound.
+    destruct Hwf; constructor; intros; simpl.
+    repeat constructor; eauto using wff_in_impl_Proper.
+  Qed.
+
+  (** We can squash [a -> b -> c] into [a -> c] if [min a b c = min a
+      c], i.e., if the narrowest type we pass through in the original
+      case is the same as the narrowest type we pass through in the
+      new case. *)
+  Definition squash_cast {var} (a b c : base_type) : @exprf base_type op var (Tbase a) -> @exprf base_type op var (Tbase c)
+    := if base_type_beq (base_type_min b (base_type_min a c)) (base_type_min a c)
+       then SmartCast_base
+       else fun x => Op (Cast b c) (Op (Cast a b) x).
+  Fixpoint maybe_push_cast {var t} (v : @exprf base_type op var t) : option (@exprf base_type op var t)
+    := match v in exprf _ _ t return option (exprf _ _ t) with
+       | Var _ _ as v'
+         => Some v'
+       | Op t1 tR opc args
+         => match opc in op src dst return exprf _ _ src -> option (exprf _ _ dst) with
+            | Cast b c
+              => fun args
+                 => match @maybe_push_cast _ _ args with
+                    | Some (Op _ _ opc' args')
+                      => match opc' in op src' dst' return exprf _ _ src' -> option (exprf _ _ (Tbase c)) with
+                         | Cast a b
+                           => fun args''
+                              => Some (squash_cast a b c args'')
+                         | OpConst _ v
+                           => fun args''
+                              => Some (SmartCast_base (Op (OpConst v) TT))
+                         | _ => fun _ => None
+                         end args'
+                    | Some (Var _ v as v') => Some (SmartCast_base v')
+                    | Some _ => None
+                    | None => None
+                    end
+            | OpConst _ v
+              => fun _ => Some (Op (OpConst v) TT)
+            | _ => fun _ => None
+            end args
+       | Pair _ _ _ _
+       | LetIn _ _ _ _
+       | TT
+         => None
+       end.
+  Definition push_cast {var t} : @exprf base_type op var t -> inline_directive (op:=op) (var:=var) t
+    := match t with
+       | Tbase _ => fun v => match maybe_push_cast v with
+                             | Some e => inline e
+                             | None => default_inline v
+                             end
+       | _ => default_inline
+       end.
+
+  (*Definition mapf_interpToZ_T (T : flat_type base_type) : flat_type base_type
+    :=
+*)
+  Definition mapf_interpToZ {T} : interp_flat_type Syntax.interp_base_type T -> interp_flat_type (fun _ => Z) T
+    := SmartVarfMap (fun _ => interpToZ).
+  Definition mapf_interp_new_flat_typeToZ {T v} : interp_flat_type Syntax.interp_base_type (@new_flat_type T v) -> interp_flat_type (fun _ => Z) T
+    := SmartFlatTypeMapUnInterp2 (f:=fun _ _ => Tbase _) (fun _ _ => interpToZ).
+
+  Lemma mapf_interpToZ_Pair {A B} x
+    : @mapf_interpToZ (Prod A B) x = (mapf_interpToZ (fst x), mapf_interpToZ (snd x)).
+  Proof. reflexivity. Qed.
+  Lemma mapf_interp_new_flat_typeToZ_Pair {A B} v e
+    : @mapf_interp_new_flat_typeToZ (Prod A B) v e = (mapf_interp_new_flat_typeToZ (fst e), mapf_interp_new_flat_typeToZ (snd e)).
+  Proof. reflexivity. Qed.
+
+  (** TODO: move me *)
+
+  Lemma interpf_maybe_push_cast t (e1 e2 : exprf base_type op t)
+        (H : maybe_push_cast e1 = Some e2)
+    : interpf Syntax.interp_op e1 = interpf Syntax.interp_op e2.
+  Proof.
+    revert dependent e2; induction e1; intro e2;
+      try (preinvert_one_type e2; intros ? e2); destruct e2;
+        try exact I;
+        repeat match goal with
+               | _ => intro
+               | _ => reflexivity
+               | [ H : forall e, Some _ = Some e -> _ |- _ ] => specialize (H _ eq_refl)
+               | [ H : base_type_beq _ _ = true |- _ ] => apply internal_base_type_dec_bl in H
+               | _ => progress subst
+               | _ => progress inversion_option
+               | _ => progress inversion_sigma
+               | _ => progress inversion_prod
+               | _ => progress inversion_expr
+               | _ => progress simpl in *
+               | _ => congruence
+               | _ => progress break_match_hyps
+               | _ => progress break_innermost_match_step
+               | _ => progress invert_match_op
+               | _ => progress invert_match_expr
+               | _ => progress unfold SmartCast_base, squash_cast in *
+               | _ => rewrite_hyp !*
+               | _ => rewrite cast_const_id in *
+               | _ => rewrite cast_const_idempotent by assumption
+               end.
+  Qed.
+
+  Lemma interpf_push_cast t (e : exprf base_type op t)
+    : interpf Syntax.interp_op (exprf_of_inline_directive (push_cast e)) = interpf Syntax.interp_op e.
+  Proof.
+    unfold push_cast;
+      break_match; try reflexivity; simpl; [].
+    symmetry; apply (@interpf_maybe_push_cast (Tbase _)); assumption.
+  Qed.
+
+  Local Hint Resolve interpf_push_cast.
+
+  Local Hint Constructors wff.
+
+  Local Ltac t_pair :=
+    repeat first [ exact I
+                 | intro
+                 | progress subst
+                 | progress destruct_head' False
+                 | progress destruct_head' sig
+                 | progress destruct_head' and
+                 | progress inversion_option
+                 | progress inversion_sigma
+                 | progress inversion_prod
+                 | progress break_match
+                 | progress simpl in *
+                 | progress inversion_wf ].
+
+  Lemma wff_SmartCast_base {var1 var2} G A A' e1 e2
+        (Hwf : wff G e1 e2)
+    : wff G (@SmartCast_base var1 A A' e1) (@SmartCast_base var2 A A' e2).
+  Proof.
+    unfold SmartCast_base; break_match; auto.
+  Qed.
+
+  Local Hint Resolve @wff_SmartCast_base.
+
+  Local Hint Extern 2 => progress simpl.
+
+  Lemma wff_PairCast {var1 var2} G a b a' b'
+        (e1 e2 : exprf base_type op (Tbase a * Tbase b))
+        (Hwf : wff (var1:=var1) (var2:=var2) G e1 e2)
+    : wff (t:=Prod (Tbase a') (Tbase b')) G (PairCast e1) (PairCast e2).
+  Proof.
+    apply wff_encode in Hwf; unfold wff_code in *;
+      preinvert_one_type e1; intros ? e1; destruct e1; try exact I; t_pair;
+        preinvert_one_type e2; intros ? e2; destruct e2; try exact I; t_pair;
+          repeat constructor; eauto 6.
+  Qed.
+
+  Local Hint Resolve wff_PairCast.
+
+  Lemma wff_QuadCast {var1 var2} G a b c d a' b' c' d'
+        (e1 e2 : exprf base_type op (Tbase a * Tbase b * Tbase c * Tbase d))
+        (Hwf : wff (var1:=var1) (var2:=var2) G e1 e2)
+    : wff G (@QuadCast var1 a b c d a' b' c' d' e1) (QuadCast e2).
+  Proof.
+    apply wff_encode in Hwf; unfold wff_code in *;
+      repeat match goal with
+             | [ e : exprf _ _ (_ * _) |- _ ]
+               => preinvert_one_type e; intros ? e; destruct e; try exact I; t_pair
+             end;
+      repeat constructor; eauto 10.
+  Qed.
+
+  Local Hint Resolve wff_QuadCast.
+
+  Lemma wff_cast_bound_op {ovar1 ovar2} G src1 dst1 src2 dst2
+        (opc1 : op src1 dst1) (opc2 : op src2 dst2)
+        (e1 e2 : exprf base_type op src1)
+        (args2 : interp_flat_type interp_base_type src2)
+        (Hwf : wff (var1:=ovar1) (var2:=ovar2) G e1 e2)
+    : wff G (cast_bound_op opc1 opc2 e1 args2) (cast_bound_op opc1 opc2 e2 args2).
+  Proof.
+    destruct opc1, opc2; simpl; auto;
+      unfold SmartCast_op1, SmartCast_op2, SmartCast_op4, SmartCast_base; break_match; subst;
+        trivial;
+        try constructor; trivial; eauto.
+  Qed.
+
+  Local Hint Resolve wff_cast_bound_op : wf.
+
+  Local Hint Resolve Wf_Linearize Wf_SmartBound Wf_MapInterpCast : wf.
+
+  Lemma interpf_SmartCast_base {A A'} e
+    : interpf (@Syntax.interp_op) (@SmartCast_base _ A A' e) = cast_const (interpf (@Syntax.interp_op) e).
+  Proof.
+    unfold SmartCast_base; break_match; rewrite ?cast_const_id; reflexivity.
+  Qed.
+
+  Lemma interpf_PairCast {A B A' B'} e
+    : interpf (@Syntax.interp_op) (@PairCast _ A B A' B' e)
+      = let ev := interpf (@Syntax.interp_op) e in
+        (cast_const (fst ev), cast_const (snd ev)).
+  Proof.
+    invert_expr; break_innermost_match; try exact I; simpl;
+      cbv [LetIn.Let_In];
+      rewrite ?interpf_SmartCast_base;
+      reflexivity.
+  Qed.
+
+  Lemma interpf_QuadCast {A B C D A' B' C' D'} e
+    : interpf (@Syntax.interp_op) (@QuadCast _ A B C D A' B' C' D' e)
+      = let ev := interpf (@Syntax.interp_op) e in
+        (cast_const (fst (fst (fst ev))),
+         cast_const (snd (fst (fst ev))),
+         cast_const (snd (fst ev)),
+         cast_const (snd ev)).
+  Proof.
+    repeat first [ exact I
+                 | reflexivity
+                 | rewrite !interpf_SmartCast_base
+                 | progress cbv [LetIn.Let_In]
+                 | progress simpl
+                 | progress break_innermost_match
+                 | progress invert_expr ].
+  Qed.
+
+  Lemma interpf_PairCast_uniform {A A'} e
+    : interpf (@Syntax.interp_op) (@PairCast _ A A A' A' e)
+      = SmartVarfMap (fun t => cast_const) (interpf (@Syntax.interp_op) e).
+  Proof. rewrite interpf_PairCast; reflexivity. Qed.
+
+  Lemma interpf_QuadCast_uniform {A A'} e
+    : interpf (@Syntax.interp_op) (@QuadCast _ A A A A A' A' A' A' e)
+      = SmartVarfMap (fun t => cast_const) (interpf (@Syntax.interp_op) e).
+  Proof. rewrite interpf_QuadCast; reflexivity. Qed.
+
+  Local Ltac rewrite_in_all lem :=
+    match goal with
+    | _ => rewrite lem
+    | [ H : _ |- _ ] => rewrite lem in H
+    end.
+
+  Local Ltac t_interpf_step :=
+    first [ reflexivity
+          | assumption
+          | progress destruct_head_hnf' unit
+          | progress destruct_head_hnf' and
+          | progress rewrite_new_flat_type_Pair
+          | rewrite_in_all SmartBoundv_Pair
+          | rewrite_in_all SmartUnboundv_Pair
+          | rewrite_in_all SmartPairf_Pair
+          | rewrite_in_all interpf_SmartCast_base
+          | rewrite_in_all map_cast_const_Pair
+          | rewrite_in_all map_uncast_const_Pair
+          | rewrite_in_all mapf_interpToZ_Pair
+          | rewrite_in_all mapf_interp_new_flat_typeToZ_Pair
+          | rewrite Z2Nat.id by auto with zarith
+          | progress split_andb
+          | rewrite_hyp !*
+          | progress (simpl @fst; simpl @snd)
+          | progress break_match_hyp
+          | progress subst
+          | progress break_innermost_match_step
+          | progress Z.ltb_to_lt
+          | rewrite_in_all Z.pow_Zpow
+          | omega ].
+
+  Lemma interpf_SmartPairf_SmartBoundv {t} bounds e
+    : interpf (@Syntax.interp_op) (SmartPairf (@SmartBoundv (@Syntax.interp_base_type) t bounds e))
+      = map_cast_const bounds e.
+  Proof.
+    induction t;
+      repeat first [ t_interpf_step
+                   | progress simpl in *
+                   | progress unfold SmartPairf, SmartBoundv, SmartFlatTypeMap2 ].
+  Qed.
+
+  Lemma interpf_SmartPairf_SmartUnboundv {t} bounds e
+    : interpf (@Syntax.interp_op) (SmartPairf (@SmartUnboundv (@Syntax.interp_base_type) t bounds e))
+      = map_uncast_const bounds e.
+  Proof.
+    induction t;
+      repeat first [ t_interpf_step
+                   | progress simpl in *
+                   | progress unfold SmartPairf, SmartUnboundv, SmartFlatTypeMap2 ].
+  Qed.
+
+  Local Arguments Z.add !_ !_.
+  Local Existing Instances Z.add_le_Proper Z.sub_le_eq_Proper Z.log2_up_le_Proper Z.pow_Zpos_le_Proper.
+  Lemma mapf_interp_new_flat_typeToZ__map_cast_const {t} bounds e
+        (Hbounded : is_bounded_by e bounds)
+    : mapf_interp_new_flat_typeToZ (@map_cast_const t bounds e)
+      = mapf_interpToZ e.
+  Proof.
+    induction t;
+      repeat first [ t_interpf_step
+                   | progress simpl in *
+                   | progress unfold map_cast_const, mapf_interp_new_flat_typeToZ
+                   | progress unfold is_bounded_by in *
+                   | progress unfold mapf_interpToZ, SmartVarfMap in *
+                   | progress unfold cast_const, bounds_to_base_type'
+                   | rewrite wordToZ_ZToWord
+                   | split; [ reflexivity | ]
+                   | match goal with
+                     | [ |- (?x < ?y)%Z ]
+                       => cut (x <= y - 1)%Z; [ omega | ]
+                     end
+                   | rewrite <- !Z.log2_up_le_full
+                   | progress unfold is_bounded_by', is_bounded_byb in * ].
+  Qed.
+
+
+  Lemma InterpSmartBound t e input_bounds
+        (Hwf : Wf e)
+    : forall (x : interp_flat_type Syntax.interp_base_type (new_flat_type (t:=domain t) input_bounds)),
+      is_bounded_by (map_uncast_const input_bounds x) input_bounds
+      -> mapf_interp_new_flat_typeToZ (Interp (@Syntax.interp_op) (SmartBound e input_bounds) x)
+         = mapf_interpToZ (Interp (@Syntax.interp_op) e (map_uncast_const input_bounds x)).
+  Proof.
+    unfold SmartBound, Interp; simpl.
+    cbv [LetIn.Let_In]; intros x H.
+    rewrite interpf_SmartPairf_SmartBoundv, interpf_SmartPairf_SmartUnboundv, interpf_invert_Abs, mapf_interp_new_flat_typeToZ__map_cast_const; [ reflexivity | ].
+    fold (@Interp _ _ _ (@interp_op) _ e).
+    fold (@Interp _ _ _ (@Syntax.interp_op) _ e).
+    apply InterpWf; [ | assumption.. ].
+    intros src dst op sv1 sv2.
+    fold (is_bounded_by sv1 sv2).
+    fold (is_bounded_by (Syntax.interp_op src dst op sv1) (interp_op op sv2)).
+    apply is_bounded_by_interp_op.
+  Qed.
+
+  Lemma interpf_SmartCast_op1 {T1 T2} (opc : forall t, op (Tbase t) (Tbase t)) args1 args2
+        (HopcZ : forall T2 x xb zb,
+            is_bounded_by (T:=Tbase TZ) x (Some xb)
+            -> interp_op (opc T2) (Some xb) = Some zb
+            -> FixedWordSizes.wordToZ (Syntax.interp_op _ _ (opc (TWord (Z.to_nat (Z.log2_up (Z.log2_up (Z.max (1 + upper xb) (1 + upper zb))))))) (FixedWordSizes.ZToWord x))
+               = Syntax.interp_op _ _ (opc TZ) x)
+        (Hb : is_bounded_by (interpf (@Syntax.interp_op) args1) args2)
+    : interpf (@Syntax.interp_op) (@SmartCast_op1 _ T1 T2 opc args1 args2)
+      = cast_const (Syntax.interp_op _ _ (opc TZ) (SmartVarfMap (fun t => @cast_const t TZ) (interpf (@Syntax.interp_op) args1))).
+  Proof.
+    unfold SmartCast_op1.
+    unfold is_bounded_by, interp_flat_type_rel_pointwise, interp_flat_type_rel_pointwise_gen_Prop, is_bounded_by', is_bounded_byb in *.
+    rewrite interpf_SmartCast_base; simpl.
+    repeat unfold bounds3_to_base_type, bounds2_to_base_type, bounds_to_base_type, bounds_to_base_type', cast_const, ZToInterp, interpToZ; simpl.
+    unfold base_type_max.
+    unfold SmartVarfMap; simpl.
+    unfold bit_width_of_base_type in *.
+    rewrite interpf_SmartCast_base.
+    repeat (break_innermost_match_step; simpl; try reflexivity);
+      destruct_head' and;
+      split_andb;
+      generalize dependent (interpf Syntax.interp_op args1); clear args1; intros;
+        simpl in *;
+        rewrite <- !Z2Nat.inj_max, !Z.max_log2_up;
+        erewrite HopcZ by (rewrite_hyp !*; reflexivity);
+        reflexivity.
+  Qed.
+
+  Lemma interpf_SmartCast_op2 {T1 T2} (opc : forall t, op (Tbase t * Tbase t) (Tbase t)) args1 args2
+        (HopcZ : forall T2 x y xb yb zb,
+            is_bounded_by (T:=Prod (Tbase TZ) (Tbase TZ)) (x, y)%core (Some xb, Some yb)%core
+            -> interp_op (opc T2) (Some xb, Some yb) = Some zb
+            -> FixedWordSizes.wordToZ (Syntax.interp_op _ _ (opc (TWord (Z.to_nat (Z.log2_up (Z.log2_up (Z.max (Z.max (1 + upper xb) (1 + upper yb)) (1 + upper zb))))))) (FixedWordSizes.ZToWord x, FixedWordSizes.ZToWord y))
+               = Syntax.interp_op _ _ (opc TZ) (x, y))
+        (Hb : is_bounded_by (interpf (@Syntax.interp_op) args1) args2)
+    : interpf (@Syntax.interp_op) (@SmartCast_op2 _ T1 T2 opc args1 args2)
+      = cast_const (Syntax.interp_op _ _ (opc TZ) (SmartVarfMap (fun t => @cast_const t TZ) (interpf (@Syntax.interp_op) args1))).
+  Proof.
+    unfold SmartCast_op2.
+    unfold is_bounded_by, interp_flat_type_rel_pointwise, interp_flat_type_rel_pointwise_gen_Prop, is_bounded_by', is_bounded_byb in *.
+    rewrite interpf_SmartCast_base; simpl.
+    rewrite interpf_PairCast_uniform.
+    destruct_head_hnf prod.
+    repeat unfold bounds3_to_base_type, bounds2_to_base_type, bounds_to_base_type, bounds_to_base_type', cast_const, ZToInterp, interpToZ; simpl.
+    unfold base_type_max.
+    unfold SmartVarfMap; simpl.
+    unfold bit_width_of_base_type in *.
+    repeat (break_innermost_match_step; simpl; try reflexivity);
+      destruct_head' and;
+      split_andb;
+      generalize dependent (interpf Syntax.interp_op args1); clear args1; intros; destruct_head_hnf prod;
+        rewrite <- !Z2Nat.inj_max, !Z.max_log2_up;
+        erewrite HopcZ by (eassumption || rewrite_hyp !*; auto);
+        reflexivity.
+  Qed.
+
+  Lemma interpf_SmartCast_op4 {T1 T2} (opc : forall t, op (Tbase t * Tbase t * Tbase t * Tbase t) (Tbase t)) args1 args2
+        (HopcZ : forall T2 x y z w xb yb zb wb ob,
+            is_bounded_by (T:=Prod (Prod (Prod (Tbase TZ) (Tbase TZ)) (Tbase TZ)) (Tbase TZ))
+                          (x, y, z, w)%core (Some xb, Some yb, Some zb, Some wb)%core
+            -> interp_op (opc T2) (Some xb, Some yb, Some zb, Some wb) = Some ob
+            -> FixedWordSizes.wordToZ (Syntax.interp_op _ _ (opc (TWord (Z.to_nat (Z.log2_up (Z.log2_up (Z.max (Z.max (Z.max (1 + upper xb) (1 + upper yb)) (Z.max (1 + upper zb) (1 + upper wb))) (1 + upper ob)))))))
+                                                        (FixedWordSizes.ZToWord x, FixedWordSizes.ZToWord y, FixedWordSizes.ZToWord z, FixedWordSizes.ZToWord w))
+               = Syntax.interp_op _ _ (opc TZ) (x, y, z, w))
+        (Hb : is_bounded_by (interpf (@Syntax.interp_op) args1) args2)
+    : interpf (@Syntax.interp_op) (@SmartCast_op4 _ T1 T2 opc args1 args2)
+      = cast_const (Syntax.interp_op _ _ (opc TZ) (SmartVarfMap (fun t => @cast_const t TZ) (interpf (@Syntax.interp_op) args1))).
+  Proof.
+    unfold SmartCast_op4.
+    unfold is_bounded_by, interp_flat_type_rel_pointwise, interp_flat_type_rel_pointwise_gen_Prop, is_bounded_by', is_bounded_byb in *.
+    rewrite interpf_SmartCast_base; simpl.
+    rewrite interpf_QuadCast_uniform.
+    destruct_head_hnf prod.
+    repeat unfold bounds5_to_base_type, bounds4_to_base_type, bounds3_to_base_type, bounds2_to_base_type, bounds_to_base_type, bounds_to_base_type', cast_const, ZToInterp, interpToZ; simpl.
+    unfold base_type_max.
+    unfold SmartVarfMap; simpl.
+    unfold bit_width_of_base_type in *.
+    repeat (break_innermost_match_step; simpl; try reflexivity);
+      destruct_head' and;
+      split_andb;
+      generalize dependent (interpf Syntax.interp_op args1); clear args1; intros; destruct_head_hnf prod;
+        rewrite <- !Z2Nat.inj_max, !Z.max_log2_up;
+        erewrite HopcZ by (eassumption || rewrite_hyp !*; auto);
+        reflexivity.
+  Qed.
+
+    Lemma interpf_cast_bound_op G t0 tR (opc : op t0 tR)
+        (ein eout ebounds : exprf base_type op t0)
+        (HG : forall (t : base_type) (x : Syntax.interp_base_type t) (x' : interp_base_type t),
+            List.In (existT _ t (x, x')) G
+            -> is_bounded_by' x x')
+        (Hwf : wff G ein ebounds)
+        (He : interpf Syntax.interp_op ein = interpf Syntax.interp_op eout)
+        (Hbounds_are_good : bounds_are_good (interpf (@interp_op) (Op opc ebounds)))
+    : interpf Syntax.interp_op (cast_bound_op opc opc eout (interpf (@interp_op) ebounds))
+      = interpf Syntax.interp_op (Op opc ein).
+  Proof.
+    assert (Hb : is_bounded_by (interpf Syntax.interp_op (Op opc ein)) (interpf (@interp_op) (Op opc ebounds)))
+      by (eapply interpf_wff; eauto; apply is_bounded_by_interp_op).
+    assert (Hb0 : is_bounded_by (interpf Syntax.interp_op ein) (interpf (@interp_op) ebounds))
+      by (eapply interpf_wff; eauto; apply is_bounded_by_interp_op).
+    destruct opc;
+      repeat first [ intro
+                   | reflexivity
+                   | progress subst
+                   | progress destruct_head' and
+                   | solve [ rewrite_hyp <- ?*; eapply interpf_wff; [ .. | eassumption ]; eauto;
+                             apply is_bounded_by_interp_op
+                           | inversion_wf; eauto ]
+                   | rewrite interpf_SmartCast_base
+                   | rewrite interpf_SmartCast_op1
+                   | rewrite interpf_SmartCast_op2
+                   | rewrite interpf_SmartCast_op4
+                   | rewrite_hyp !*
+                   | progress simpl in *
+                   | progress break_innermost_match ].
+    all:unfold is_bounded_by', is_bounded_byb in *.
+    all:simpl in *.
+    { repeat first [ progress unfold add, add' in *
+                   | progress unfold t_map2, SmartBuildBounds, bound_is_good, bound_is_goodb in *
+                   | progress subst
+                   | progress inversion_option
+                   | progress split_andb
+                   | progress break_match_hyps
+                   | progress Z.ltb_to_lt
+                   | progress simpl in *
+                   | progress rewrite_hyp <- ?*
+                   | match goal with
+                     | [ H : context[andb _ _ = false] |- _ ] => rewrite Bool.andb_false_iff in H
+                     end
+                   | progress destruct_head' or
+                   | exfalso; omega
+                   | congruence ].
+      { Local Ltac def_ZToWord_t :=
+          first [ eapply Z.le_lt_trans; [ apply Z.log2_le_mono | eassumption ]; omega ].
+        rewrite wadd_def_ZToWord by def_ZToWord_t.
+        reflexivity. } }
+    { repeat first [ progress unfold add, add' in *
+                   | progress unfold t_map2, SmartBuildBounds, bound_is_good, bound_is_goodb, bit_width_of_base_type in *
+                   | progress subst
+                   | progress inversion_option
+                   | progress split_andb
+                   | progress break_match_hyps
+                   | progress Z.ltb_to_lt
+                   | progress simpl in *
+                   | progress rewrite_hyp <- ?*
+                   | match goal with
+                     | [ H : context[andb _ _ = false] |- _ ] => rewrite Bool.andb_false_iff in H
+                     end
+                   | progress destruct_head' or
+                   | exfalso; omega
+                   | congruence ].
+      { rewrite wadd_def_ZToWord;
+          repeat rewrite !wordToZ_ZToWord.
+        reflexivity.
+        all:try split; try omega.
+        all:rewrite ?Z.pow_Zpow, ?Z2Nat.id, ?Nat2Z.inj_succ, ?Nat2Z.inj_0, <- ?Z.one_succ, <- ?Z.two_succ.
+        all:auto using Z.log2_up_nonneg.
+        all: repeat apply Z.max_case_strong; intros.
+        all: try (eapply Z.lt_le_trans; [ | rewrite <- !Z.log2_up_le_full_max; reflexivity ]).
+        all: repeat apply Z.max_case_strong; intros.
+        all: try (eapply Z.lt_le_trans; [ | rewrite <- !Z.log2_up_le_full_max; reflexivity ]).
+        all: repeat apply Z.max_case_strong; intros.
+        all: try omega.
+        all: change (2^1)%Z with 2%Z in *.
+        all: try omega.
+        all:repeat match goal with
+                   | [ H : (Z.log2_up _ <= 1)%Z |- _ ] => apply Z.log2_up_le_1 in H
+                   | [ H : (1 <= Z.log2_up _)%Z |- _ ] => apply Z.log2_up_1_le in H
+                   end.
+        all: try omega.
+        all: rewrite ?Z.log2_up_eqn by omega.
+        all: try apply Zle_lt_succ.
+        all: try apply Z.log2_le_mono.
+        all: try omega.
+        Local Open Scope Z_scope.
+        all: repeat match goal with
+                    | [ H : 1 + ?x <= 2 |- _ ] => assert (x <= 1) by omega; clear H
+                    | [ H : 1 + ?x <= 1 |- _ ] => assert (x <= 0) by omega; clear H
+                    | [ H : (?x <= 1)%Z |- _ ]
+                      => is_var x;
+                           assert (0 <= x <= 1) by omega;
+                           assert (x = 0 \/ x = 1) by omega;
+                           destruct_head' or; subst
+                    | [ H : ?x + ?y <= 1 |- _ ]
+                      => is_var x; is_var y;
+                           assert (0 <= x + y <= 1) by omega;
+                           assert ((x = 0 /\ y = 0) \/ (x = 0 /\ y = 1) \/ (x = 1 /\ y = 0)) by omega;
+                           destruct_head' or; destruct_head' and; subst
+                    | [ H : ?x <= 0 |- _ ]
+                      => is_var x;
+                           assert (x = 0) by omega;
+                           destruct_head' or; subst
+                    | [ H : ?x <= ?x |- _ ] => clear H
+                    | [ H : ?a <= ?b, H' : ?a <= ?b |- _ ] => clear H'
+                    | [ H : 0 <= 1 |- _ ] => clear H
+                    | _ => progress simpl in *
+                    | [ H : 0 <= 0 <= 1 |- _ ] => clear H
+                    | [ H : context[0 + _] |- _ ] => rewrite Z.add_0_l in H
+                    | [ H : 1 + ?x <= 1 + ?y |- _ ] => assert (x <= y) by omega; clear H
+                    | [ H : ?x <= ?x + ?y |- _ ] => assert (0 <= y) by omega; clear H
+                    | _ => omega
+                    end. }
+      { rewrite wadd_def_ZToWord;
+          repeat rewrite !wordToZ_ZToWord.
+        reflexivity.
+        all:try split; try omega.
+        all:rewrite ?Z.pow_Zpow, ?Z2Nat.id, ?Nat2Z.inj_succ, ?Nat2Z.inj_0, <- ?Z.one_succ, <- ?Z.two_succ.
+        all:auto using Z.log2_up_nonneg.
+        all: repeat apply Z.max_case_strong; intros.
+        all: try (eapply Z.lt_le_trans; [ | rewrite <- !Z.log2_up_le_full_max; reflexivity ]).
+        all: repeat apply Z.max_case_strong; intros.
+        all: try (eapply Z.lt_le_trans; [ | rewrite <- !Z.log2_up_le_full_max; reflexivity ]).
+        all: repeat apply Z.max_case_strong; intros.
+        all: try omega.
+        all: change (2^1) with 2 in *.
+        all: try omega.
+        all:repeat match goal with
+                   | [ H : Z.log2_up _ <= 1 |- _ ] => apply Z.log2_up_le_1 in H
+                   | [ H : 1 <= Z.log2_up _ |- _ ] => apply Z.log2_up_1_le in H
+                   end.
+        all: try omega.
+        all: rewrite ?Z.log2_up_eqn by omega.
+        all: try apply Zle_lt_succ.
+        all: try apply Z.log2_le_mono.
+        all: try omega.
+        all: repeat match goal with
+                    | [ H : 1 + ?x <= 2 |- _ ] => assert (x <= 1) by omega; clear H
+                    | [ H : 1 + ?x <= 1 |- _ ] => assert (x <= 0) by omega; clear H
+                    | [ H : ?x <= 1 |- _ ]
+                      => is_var x;
+                           assert (0 <= x <= 1) by omega;
+                           assert (x = 0 \/ x = 1) by omega;
+                           destruct_head' or; subst
+                    | [ H : ?x + ?y <= 1 |- _ ]
+                      => is_var x; is_var y;
+                           assert (0 <= x + y <= 1) by omega;
+                           assert ((x = 0 /\ y = 0) \/ (x = 0 /\ y = 1) \/ (x = 1 /\ y = 0)) by omega;
+                           destruct_head' or; destruct_head' and; subst
+                    | [ H : ?x <= 0 |- _ ]
+                      => is_var x;
+                           assert (x = 0) by omega;
+                           destruct_head' or; subst
+                    | [ H : ?x <= ?x |- _ ] => clear H
+                    | [ H : ?a <= ?b, H' : ?a <= ?b |- _ ] => clear H'
+                    | [ H : 0 <= 1 |- _ ] => clear H
+                    | _ => progress simpl in *
+                    | [ H : 0 <= 0 <= 1 |- _ ] => clear H
+                    | [ H : context[0 + _] |- _ ] => rewrite Z.add_0_l in H
+                    | [ H : 1 + ?x <= 1 + ?y |- _ ] => assert (x <= y) by omega; clear H
+                    | [ H : ?x <= ?x + ?y |- _ ] => assert (0 <= y) by omega; clear H
+                    | _ => omega
+                    end. }
+      { rewrite wadd_def_ZToWord;
+          repeat rewrite !wordToZ_ZToWord.
+        reflexivity.
+        all:try split; try omega.
+        all:rewrite ?Z.pow_Zpow, ?Z2Nat.id, ?Nat2Z.inj_succ, ?Nat2Z.inj_0, <- ?Z.one_succ, <- ?Z.two_succ.
+        all:auto using Z.log2_up_nonneg.
+        all: repeat apply Z.max_case_strong; intros.
+        all: try (eapply Z.lt_le_trans; [ | rewrite <- !Z.log2_up_le_full_max; reflexivity ]).
+        all: repeat apply Z.max_case_strong; intros.
+        all: try (eapply Z.lt_le_trans; [ | rewrite <- !Z.log2_up_le_full_max; reflexivity ]).
+        all: repeat apply Z.max_case_strong; intros.
+        all: try omega.
+        all: change (2^1) with 2 in *.
+        all: try omega.
+        all:repeat match goal with
+                   | [ H : Z.log2_up _ <= 1 |- _ ] => apply Z.log2_up_le_1 in H
+                   | [ H : 1 <= Z.log2_up _ |- _ ] => apply Z.log2_up_1_le in H
+                   end.
+        all: try omega.
+        all: rewrite ?Z.log2_up_eqn by omega.
+        all: try apply Zle_lt_succ.
+        all: try apply Z.log2_le_mono.
+        all: try omega.
+        all: repeat match goal with
+                    | [ H : 1 + ?x <= 2 |- _ ] => assert (x <= 1) by omega; clear H
+                    | [ H : 1 + ?x <= 1 |- _ ] => assert (x <= 0) by omega; clear H
+                    | [ H : ?x <= 1 |- _ ]
+                      => is_var x;
+                           assert (0 <= x <= 1) by omega;
+                           assert (x = 0 \/ x = 1) by omega;
+                           destruct_head' or; subst
+                    | [ H : ?x + ?y <= 1 |- _ ]
+                      => is_var x; is_var y;
+                           assert (0 <= x + y <= 1) by omega;
+                           assert ((x = 0 /\ y = 0) \/ (x = 0 /\ y = 1) \/ (x = 1 /\ y = 0)) by omega;
+                           destruct_head' or; destruct_head' and; subst
+                    | [ H : ?x <= 0 |- _ ]
+                      => is_var x;
+                           assert (x = 0) by omega;
+                           destruct_head' or; subst
+                    | [ H : ?x <= ?x |- _ ] => clear H
+                    | [ H : ?a <= ?b, H' : ?a <= ?b |- _ ] => clear H'
+                    | [ H : 0 <= 1 |- _ ] => clear H
+                    | _ => progress simpl in *
+                    | [ H : 0 <= 0 <= 1 |- _ ] => clear H
+                    | [ H : context[0 + _] |- _ ] => rewrite Z.add_0_l in H
+                    | [ H : 1 + ?x <= 1 + ?y |- _ ] => assert (x <= y) by omega; clear H
+                    | [ H : ?x <= ?x + ?y |- _ ] => assert (0 <= y) by omega; clear H
+                    | _ => omega
+                    end. }
+      { rewrite wadd_def_ZToWord;
+          repeat rewrite !wordToZ_ZToWord.
+        reflexivity.
+        all:try split; try omega.
+        all:rewrite ?Z.pow_Zpow, ?Z2Nat.id, ?Nat2Z.inj_succ, ?Nat2Z.inj_0, <- ?Z.one_succ, <- ?Z.two_succ.
+        all:auto using Z.log2_up_nonneg.
+        all: repeat apply Z.max_case_strong; intros.
+        all: try (eapply Z.lt_le_trans; [ | rewrite <- !Z.log2_up_le_full_max; reflexivity ]).
+        all: repeat apply Z.max_case_strong; intros.
+        all: try (eapply Z.lt_le_trans; [ | rewrite <- !Z.log2_up_le_full_max; reflexivity ]).
+        all: repeat apply Z.max_case_strong; intros.
+        all: try omega.
+        all: change (2^1) with 2 in *.
+        all: try omega.
+        all:repeat match goal with
+                   | [ H : Z.log2_up _ <= 1 |- _ ] => apply Z.log2_up_le_1 in H
+                   | [ H : 1 <= Z.log2_up _ |- _ ] => apply Z.log2_up_1_le in H
+                   end.
+        all: try omega.
+        all: rewrite ?Z.log2_up_eqn by omega.
+        all: try apply Zle_lt_succ.
+        all: try apply Z.log2_le_mono.
+        all: try omega.
+        all: repeat match goal with
+                    | [ H : 1 + ?x <= 2 |- _ ] => assert (x <= 1) by omega; clear H
+                    | [ H : 1 + ?x <= 1 |- _ ] => assert (x <= 0) by omega; clear H
+                    | [ H : ?x <= 1 |- _ ]
+                      => is_var x;
+                           assert (0 <= x <= 1) by omega;
+                           assert (x = 0 \/ x = 1) by omega;
+                           destruct_head' or; subst
+                    | [ H : ?x + ?y <= 1 |- _ ]
+                      => is_var x; is_var y;
+                           assert (0 <= x + y <= 1) by omega;
+                           assert ((x = 0 /\ y = 0) \/ (x = 0 /\ y = 1) \/ (x = 1 /\ y = 0)) by omega;
+                           destruct_head' or; destruct_head' and; subst
+                    | [ H : ?x <= 0 |- _ ]
+                      => is_var x;
+                           assert (x = 0) by omega;
+                           destruct_head' or; subst
+                    | [ H : ?x <= ?x |- _ ] => clear H
+                    | [ H : ?a <= ?b, H' : ?a <= ?b |- _ ] => clear H'
+                    | [ H : 0 <= 1 |- _ ] => clear H
+                    | _ => progress simpl in *
+                    | [ H : 0 <= 0 <= 1 |- _ ] => clear H
+                    | [ H : context[0 + _] |- _ ] => rewrite Z.add_0_l in H
+                    | [ H : 1 + ?x <= 1 + ?y |- _ ] => assert (x <= y) by omega; clear H
+                    | [ H : ?x <= ?x + ?y |- _ ] => assert (0 <= y) by omega; clear H
+                    | _ => omega
+                    end. } }
+  Admitted.
+
+  Lemma is_bounded_by_cast_bound_op G t0 tR (opc : op t0 tR)
+        (ein eout ebounds : exprf base_type op t0)
+        (HG : forall (t : base_type) (x : Syntax.interp_base_type t) (x' : interp_base_type t),
+            List.In (existT _ t (x, x')) G
+            -> is_bounded_by' x x')
+        (Hwf : wff G ein ebounds)
+        (He : interpf Syntax.interp_op ein = interpf Syntax.interp_op eout)
+        (Hbounds_are_good : bounds_are_good (interpf (@interp_op) (Op opc ebounds)))
+    : is_bounded_by
+        (interpf Syntax.interp_op (cast_bound_op opc opc eout (interpf (@interp_op) ebounds)))
+        (interpf (@interp_op) (Op opc ebounds)).
+  Proof.
+    erewrite interpf_cast_bound_op by eassumption.
+    simpl; apply is_bounded_by_interp_op.
+    eapply interpf_wff; eauto; apply is_bounded_by_interp_op.
+  Qed.
+
+  Lemma MapBounds_correct_and_bounded {t}
+        (e : Expr base_type op t)
+        (Hwf : Wf e)
+        (input_bounds : interp_flat_type interp_base_type (domain t))
+        (output_bounds := ComputeBounds e input_bounds)
+        (e' := MapBounds e input_bounds)
+        (Hgood : bounds_are_recursively_good
+                   (@interp_op) bound_is_good
+                   (invert_Abs (e interp_base_type) input_bounds))
+    : forall x y,
+      map_uncast_const input_bounds x = y
+      -> is_bounded_by y input_bounds
+      -> is_bounded_by (Interp (@Syntax.interp_op) e (map_uncast_const _ x)) output_bounds
+         /\ mapf_interp_new_flat_typeToZ (Interp (@Syntax.interp_op) e' x)
+            = mapf_interpToZ (Interp (@Syntax.interp_op) e y).
+  Proof.
+    intros x y ? Hb; subst y output_bounds e'.
+    unfold MapBounds, ComputeBounds.
+    rewrite InterpExprEta.
+    rewrite Interp_InlineConstGen by auto with wf.
+    rewrite Interp_Linearize.
+    rewrite InterpSmartBound by auto with wf.
+    erewrite InterpMapInterpCast with (R':=@is_bounded_by')
+      by solve [ eauto with wf
+               | intros; eapply is_bounded_by_cast_bound_op; eauto
+               | intros; eapply interpf_cast_bound_op; eauto ].
+    split; [ | reflexivity ].
+    eapply InterpWf; eauto; apply is_bounded_by_interp_op.
+  Qed.*)
+
+
+(*
+  Definition is_bounded_and_correct {T1 T2 TB}
+             (interpreted_val : interp_flat_type Syntax.interp_base_type T1)
+             (orig_val : interp_flat_type Syntax.interp_base_type T2)
+             (bounds : interp_flat_type interp_base_type TB)
+    : Prop
+    := mapf_interpToZ interpreted_val = orig_val
+
+  (((Tuple.map (n:=k) fe25519WToZ irop = op)
+       /\ HList.hlistP (fun v => is_bounded v = true) (Tuple.map (n:=k) fe25519WToZ irop))%type)*)
+End Bounds.
