src/SpecificGen/GF25519_64Reflective/Reified/CarrySub.v
@@ -1,17 +1,16 @@
-Require Import Crypto.SpecificGen.GF25519_64Reflective.CommonBinOp.
+Require Import Crypto.SpecificGen.GF25519_64Reflective.Common.
 
 Definition rcarry_subZ_sig : rexpr_binop_sig carry_sub. Proof. reify_sig. Defined.
-Definition rcarry_subW := Eval vm_compute in rword_of_Z rcarry_subZ_sig.
-Lemma rcarry_subW_correct_and_bounded_gen : correct_and_bounded_genT rcarry_subW rcarry_subZ_sig.
-Proof. rexpr_correct. Qed.
-Definition rcarry_sub_output_bounds := Eval vm_compute in compute_bounds rcarry_subW ExprBinOp_bounds.
+Definition rcarry_subZ : Syntax.Expr _ _ _ := Eval vm_compute in proj1_sig rcarry_subZ_sig.
+Definition rcarry_subW : Syntax.Expr _ _ _ := Eval vm_compute in rexpr_select_word_sizes rcarry_subZ ExprBinOp_bounds.
+Definition rcarry_subZ_Wf : rexpr_wfT rcarry_subZ. Proof. prove_rexpr_wfT. Qed.
+Definition rcarry_sub_output_bounds
+  := Eval vm_compute in compute_bounds rcarry_subZ ExprBinOp_bounds.
 Local Obligation Tactic := intros; vm_compute; constructor.
-Program Definition rcarry_subW_correct_and_bounded
-  := ExprBinOp_correct_and_bounded
-       rcarry_subW carry_sub rcarry_subZ_sig rcarry_subW_correct_and_bounded_gen
-       _ _.
+Program Definition rcarry_subZ_correct_and_bounded
+  := rexpr_correct_and_bounded rcarry_subZ rcarry_subZ_Wf ExprBinOp_bounds.
 
 Local Open Scope string_scope.
-Compute ("Carry_Sub", compute_bounds_for_display rcarry_subW ExprBinOp_bounds).
-Compute ("Carry_Sub overflows? ", sanity_compute rcarry_subW ExprBinOp_bounds).
-Compute ("Carry_Sub overflows (error if it does)? ", sanity_check rcarry_subW ExprBinOp_bounds).
+Compute ("Carry_Sub", compute_bounds_for_display rcarry_subZ ExprBinOp_bounds).
+Compute ("Carry_Sub overflows? ", sanity_compute rcarry_subZ ExprBinOp_bounds).
+Compute ("Carry_Sub overflows (error if it does)? ", sanity_check rcarry_subZ ExprBinOp_bounds).
